<?xml version="1.0"?>


<!DOCTYPE rdf:RDF [
    <!ENTITY owl "http://www.w3.org/2002/07/owl#" >
    <!ENTITY xsd "http://www.w3.org/2001/XMLSchema#" >
    <!ENTITY rdfs "http://www.w3.org/2000/01/rdf-schema#" >
    <!ENTITY rdf "http://www.w3.org/1999/02/22-rdf-syntax-ns#" >
    <!ENTITY cdao "http://purl.obolibrary.org/obo/cdao/2012-06-06/cdao.owl" >
    <!ENTITY dla "http://www.datelife.org/vocabulary/datelifeannotation.owl#" >
]>


<rdf:RDF xmlns="http://www.datelife.org/vocabulary/datelifeannotation.owl#"
     xml:base="http://www.datelife.org/vocabulary/datelifeannotation.owl"
     xmlns:rdfs="http://www.w3.org/2000/01/rdf-schema#"
     xmlns:cdao="http://purl.obolibrary.org/obo/cdao/2012-06-06/cdao.owl"
     xmlns:dla="http://www.datelife.org/vocabulary/datelifeannotation.owl#"
     xmlns:owl="http://www.w3.org/2002/07/owl#"
     xmlns:xsd="http://www.w3.org/2001/XMLSchema#"
     xmlns:rdf="http://www.w3.org/1999/02/22-rdf-syntax-ns#">
    <owl:Ontology rdf:about="http://www.datelife.org/vocabulary/datelifeannotation.owl"/>
    


    <!-- 
    ///////////////////////////////////////////////////////////////////////////////////////
    //
    // Annotation properties
    //
    ///////////////////////////////////////////////////////////////////////////////////////
     -->

    


    <!-- 
    ///////////////////////////////////////////////////////////////////////////////////////
    //
    // Datatypes
    //
    ///////////////////////////////////////////////////////////////////////////////////////
     -->

    


    <!-- 
    ///////////////////////////////////////////////////////////////////////////////////////
    //
    // Object Properties
    //
    ///////////////////////////////////////////////////////////////////////////////////////
     -->

    


    <!-- http://www.datelife.org/vocabulary/datelifeannotation.owl#OWLObjectProperty_01339084329409002000 -->

    <owl:ObjectProperty rdf:about="&dla;OWLObjectProperty_01339084329409002000">
        <rdfs:label xml:lang="en">fcdbEntry</rdfs:label>
        <rdfs:comment xml:lang="en">A URL that links to the entry on FCDB (or for the moment the url to Date-A-Clade)</rdfs:comment>
    </owl:ObjectProperty>
    


    <!-- http://www.datelife.org/vocabulary/datelifeannotation.owl#OWLObjectProperty_01339088488288051000 -->

    <owl:ObjectProperty rdf:about="&dla;OWLObjectProperty_01339088488288051000">
        <rdfs:label xml:lang="en">pbdbEntry</rdfs:label>
        <rdfs:comment xml:lang="en">link to the PaleoBiology DB (PBDB) entry for the fossil (if available, though, this might not be entirely necessary if the calibration comes from the FCDB) </rdfs:comment>
    </owl:ObjectProperty>
    


    <!-- 
    ///////////////////////////////////////////////////////////////////////////////////////
    //
    // Data properties
    //
    ///////////////////////////////////////////////////////////////////////////////////////
     -->

    


    <!-- http://www.datelife.org/vocabulary/datelifeannotation.owl#OWLDataProperty_01339081909405100000 -->

    <owl:DatatypeProperty rdf:about="&dla;OWLDataProperty_01339081909405100000">
        <rdfs:label xml:lang="en">OWLDataProperty_01339081909405100000</rdfs:label>
        <rdfs:label xml:lang="en">nodeAge</rdfs:label>
        <rdfs:range rdf:resource="&xsd;float"/>
    </owl:DatatypeProperty>
    


    <!-- http://www.datelife.org/vocabulary/datelifeannotation.owl#OWLDataProperty_01339081918618771000 -->

    <owl:DatatypeProperty rdf:about="&dla;OWLDataProperty_01339081918618771000">
        <rdfs:label xml:lang="en">branchLengthService</rdfs:label>
        <rdfs:comment xml:lang="en">Description of the service that got the branch lengths (e.g., datalife or Congruifier)</rdfs:comment>
    </owl:DatatypeProperty>
    


    <!-- http://www.datelife.org/vocabulary/datelifeannotation.owl#OWLDataProperty_01339082300088898000 -->

    <owl:DatatypeProperty rdf:about="&dla;OWLDataProperty_01339082300088898000">
        <rdfs:label xml:lang="en">serviceOptions</rdfs:label>
        <rdfs:comment xml:lang="en">Description of the options that were used</rdfs:comment>
    </owl:DatatypeProperty>
    


    <!-- http://www.datelife.org/vocabulary/datelifeannotation.owl#OWLDataProperty_01339082334299907000 -->

    <owl:DatatypeProperty rdf:about="&dla;OWLDataProperty_01339082334299907000">
        <rdfs:label xml:lang="en">analysisDate</rdfs:label>
        <rdfs:comment xml:lang="en">Date this was done</rdfs:comment>
    </owl:DatatypeProperty>
    


    <!-- http://www.datelife.org/vocabulary/datelifeannotation.owl#OWLDataProperty_01339082529518740000 -->

    <owl:DatatypeProperty rdf:about="&dla;OWLDataProperty_01339082529518740000">
        <rdfs:label xml:lang="en">branchLengthSourceTreeCitation</rdfs:label>
    </owl:DatatypeProperty>
    


    <!-- http://www.datelife.org/vocabulary/datelifeannotation.owl#OWLDataProperty_01339082621051616000 -->

    <owl:DatatypeProperty rdf:about="&dla;OWLDataProperty_01339082621051616000">
        <rdfs:label xml:lang="en">userTreeCitation</rdfs:label>
        <rdfs:comment xml:lang="en">Citation of the tree we&#39;re dating (could be user, could from phylotastic)</rdfs:comment>
    </owl:DatatypeProperty>
    


    <!-- http://www.datelife.org/vocabulary/datelifeannotation.owl#OWLDataProperty_01339082666701394000 -->

    <owl:DatatypeProperty rdf:about="&dla;OWLDataProperty_01339082666701394000">
        <rdfs:label xml:lang="en">serviceErrors</rdfs:label>
        <rdfs:comment xml:lang="en">List of errors/problems if any</rdfs:comment>
    </owl:DatatypeProperty>
    


    <!-- http://www.datelife.org/vocabulary/datelifeannotation.owl#OWLDataProperty_01339082770152349000 -->

    <owl:DatatypeProperty rdf:about="&dla;OWLDataProperty_01339082770152349000">
        <rdfs:label xml:lang="en">treeSet</rdfs:label>
        <rdfs:comment xml:lang="en">If the tree is associated with other trees (e.g. an MCMC set of trees or multiple trees from different r8s runs) this indicates that and links it to other trees; or if tree is summary of multiple trees.</rdfs:comment>
    </owl:DatatypeProperty>
    


    <!-- http://www.datelife.org/vocabulary/datelifeannotation.owl#OWLDataProperty_01339082866422855000 -->

    <owl:DatatypeProperty rdf:about="&dla;OWLDataProperty_01339082866422855000">
        <rdfs:label xml:lang="en">nodeAge</rdfs:label>
        <rdfs:subPropertyOf rdf:resource="&owl;topDataProperty"/>
    </owl:DatatypeProperty>
    


    <!-- http://www.datelife.org/vocabulary/datelifeannotation.owl#OWLDataProperty_01339083101059928000 -->

    <owl:DatatypeProperty rdf:about="&dla;OWLDataProperty_01339083101059928000">
        <rdfs:label xml:lang="en">ageSummary</rdfs:label>
        <rdfs:comment xml:lang="en">Summary statistics of age, if derived from multiple trees</rdfs:comment>
    </owl:DatatypeProperty>
    


    <!-- http://www.datelife.org/vocabulary/datelifeannotation.owl#OWLDataProperty_01339083147370146000 -->

    <owl:DatatypeProperty rdf:about="&dla;OWLDataProperty_01339083147370146000">
        <rdfs:label xml:lang="en">meanAgeSummary</rdfs:label>
        <rdfs:comment xml:lang="en">Summary of multiple age estimates expressed as a mean.</rdfs:comment>
        <rdfs:subPropertyOf rdf:resource="&dla;OWLDataProperty_01339083101059928000"/>
        <rdfs:range rdf:resource="&xsd;float"/>
    </owl:DatatypeProperty>
    


    <!-- http://www.datelife.org/vocabulary/datelifeannotation.owl#OWLDataProperty_01339083160190079000 -->

    <owl:DatatypeProperty rdf:about="&dla;OWLDataProperty_01339083160190079000">
        <rdfs:label xml:lang="en">medianAgeSummary</rdfs:label>
        <rdfs:comment xml:lang="en">Summary of multiple age estimates expressed as a median.</rdfs:comment>
        <rdfs:subPropertyOf rdf:resource="&dla;OWLDataProperty_01339083101059928000"/>
        <rdfs:range rdf:resource="&xsd;float"/>
    </owl:DatatypeProperty>
    


    <!-- http://www.datelife.org/vocabulary/datelifeannotation.owl#OWLDataProperty_01339083179001988000 -->

    <owl:DatatypeProperty rdf:about="&dla;OWLDataProperty_01339083179001988000">
        <rdfs:label xml:lang="en">ageRangeSummary</rdfs:label>
        <rdfs:comment xml:lang="en">Summary of multiple age estimates expressed as a range.</rdfs:comment>
        <rdfs:subPropertyOf rdf:resource="&dla;OWLDataProperty_01339083101059928000"/>
    </owl:DatatypeProperty>
    


    <!-- http://www.datelife.org/vocabulary/datelifeannotation.owl#OWLDataProperty_01339083196651359000 -->

    <owl:DatatypeProperty rdf:about="&dla;OWLDataProperty_01339083196651359000">
        <rdfs:label xml:lang="en">nodeSupportValue</rdfs:label>
        <rdfs:comment xml:lang="en">Support value, if any, for the node</rdfs:comment>
    </owl:DatatypeProperty>
    


    <!-- http://www.datelife.org/vocabulary/datelifeannotation.owl#OWLDataProperty_01339083336741139000 -->

    <owl:DatatypeProperty rdf:about="&dla;OWLDataProperty_01339083336741139000">
        <rdfs:label xml:lang="en">taxonomicName</rdfs:label>
        <rdfs:comment xml:lang="en">Node name, if any, from taxonomy (e.g., Glires)</rdfs:comment>
        <rdfs:subPropertyOf rdf:resource="&owl;topDataProperty"/>
    </owl:DatatypeProperty>
    


    <!-- http://www.datelife.org/vocabulary/datelifeannotation.owl#OWLDataProperty_01339083386141541000 -->

    <owl:DatatypeProperty rdf:about="&dla;OWLDataProperty_01339083386141541000">
        <rdfs:label xml:lang="en">nodeSpecificErrors</rdfs:label>
        <rdfs:comment xml:lang="en">Per node error or cautionary messages (such as the node being made a polytomy due to dating conflicts)</rdfs:comment>
    </owl:DatatypeProperty>
    


    <!-- http://www.datelife.org/vocabulary/datelifeannotation.owl#OWLDataProperty_01339083477018513000 -->

    <owl:DatatypeProperty rdf:about="&dla;OWLDataProperty_01339083477018513000">
        <rdfs:label xml:lang="en">fossilSpecimenName</rdfs:label>
    </owl:DatatypeProperty>
    


    <!-- http://www.datelife.org/vocabulary/datelifeannotation.owl#OWLDataProperty_01339083571118690000 -->

    <owl:DatatypeProperty rdf:about="&dla;OWLDataProperty_01339083571118690000">
        <rdfs:label xml:lang="en">calibrationSource</rdfs:label>
        <rdfs:comment xml:lang="en">Name of the source of the calibration (biogeographical or secondary calibration)</rdfs:comment>
    </owl:DatatypeProperty>
    


    <!-- http://www.datelife.org/vocabulary/datelifeannotation.owl#OWLDataProperty_01339083625212709000 -->

    <owl:DatatypeProperty rdf:about="&dla;OWLDataProperty_01339083625212709000">
        <rdfs:label xml:lang="en">calibrationSummaryAge</rdfs:label>
        <rdfs:comment xml:lang="en">“Best guess” age: perhaps the mean or median age (mean makes sense for a single Bayesian run, but when aggregating data across many analyses, one really bad study could affect mean more than median)</rdfs:comment>
        <rdfs:range rdf:resource="&xsd;float"/>
    </owl:DatatypeProperty>
    


    <!-- http://www.datelife.org/vocabulary/datelifeannotation.owl#OWLDataProperty_01339083752413345000 -->

    <owl:DatatypeProperty rdf:about="&dla;OWLDataProperty_01339083752413345000">
        <rdfs:label xml:lang="en">minimumNodeAge</rdfs:label>
        <rdfs:comment xml:lang="en">Minimum age for the node from the fossil calibration (this may be a range of dates)</rdfs:comment>
        <rdfs:range rdf:resource="&xsd;float"/>
    </owl:DatatypeProperty>
    


    <!-- http://www.datelife.org/vocabulary/datelifeannotation.owl#OWLDataProperty_01339083941578052000 -->

    <owl:DatatypeProperty rdf:about="&dla;OWLDataProperty_01339083941578052000">
        <rdfs:label xml:lang="en">maximumNodeAge</rdfs:label>
        <rdfs:comment xml:lang="en">Maximum age of the node, if available (if there is a maximum age, there might be a different citation for this)</rdfs:comment>
        <rdfs:range rdf:resource="&xsd;float"/>
    </owl:DatatypeProperty>
    


    <!-- http://www.datelife.org/vocabulary/datelifeannotation.owl#OWLDataProperty_01339083971349655000 -->

    <owl:DatatypeProperty rdf:about="&dla;OWLDataProperty_01339083971349655000">
        <rdfs:label xml:lang="en">ageProbabilityDistribution</rdfs:label>
        <rdfs:comment xml:lang="en">Probability distribution for the age (perhaps in BEAST format, or a standard ontology for log normal, normal, etc.)</rdfs:comment>
    </owl:DatatypeProperty>
    


    <!-- http://www.datelife.org/vocabulary/datelifeannotation.owl#OWLDataProperty_01339084076460436000 -->

    <owl:DatatypeProperty rdf:about="&dla;OWLDataProperty_01339084076460436000">
        <rdfs:label xml:lang="en">fcdbCitation</rdfs:label>
        <rdfs:comment xml:lang="en">If the fossil is from FCDB, then a link to citation for the FCDB</rdfs:comment>
    </owl:DatatypeProperty>
    


    <!-- http://www.datelife.org/vocabulary/datelifeannotation.owl#OWLDataProperty_01339084241757702000 -->

    <owl:DatatypeProperty rdf:about="&dla;OWLDataProperty_01339084241757702000">
        <rdfs:label xml:lang="en">fossilCitation</rdfs:label>
        <rdfs:comment xml:lang="en">Citations associated with the fossil (e.g. the citation describing the fossil, this might not be available from calibration database)</rdfs:comment>
    </owl:DatatypeProperty>
    


    <!-- http://www.datelife.org/vocabulary/datelifeannotation.owl#OWLDataProperty_01339084279353898000 -->

    <owl:DatatypeProperty rdf:about="&dla;OWLDataProperty_01339084279353898000">
        <rdfs:label xml:lang="en">validationCitation</rdfs:label>
        <rdfs:comment xml:lang="en">If the fossil is from the Fossil Calibration DataBase (FCDB), then there will a citation validating it as a fossil calibration (most likely published in Paleontologica Electronica)</rdfs:comment>
    </owl:DatatypeProperty>
</rdf:RDF>



<!-- Generated by the OWL API (version 3.2.3.1824) http://owlapi.sourceforge.net -->

